pKVM-simplified-model/theories/main.v
@@ -18,27 +18,27 @@ Require Export step.
 
 Definition take_step
   (trans : ghost_simplified_model_transition) 
-  (st : ghost_simplified_memory) : 
+  (gsm : ghost_simplified_model) : 
   ghost_simplified_model_result :=
   match trans.(gsmt_data) with
   | GSMDT_TRANS_MEM_WRITE wd =>
-      step_write trans.(gsmt_thread_identifier) wd st
+      step_write trans.(gsmt_thread_identifier) wd gsm
   | GSMDT_TRANS_MEM_ZALLOC zd =>
-      step_zalloc zd st
+      step_zalloc zd gsm
   | GSMDT_TRANS_MEM_READ rd =>
-      step_read trans.(gsmt_thread_identifier) rd st
+      step_read trans.(gsmt_thread_identifier) rd gsm
   | GSMDT_TRANS_BARRIER ( Barrier_DSB dsb_data) =>
-      step_dsb trans.(gsmt_thread_identifier) dsb_data st
+      step_dsb trans.(gsmt_thread_identifier) dsb_data gsm
   | GSMDT_TRANS_BARRIER (_) =>
-      {| gsmsr_log := []; gsmsr_data := Ok _ _ st |} (* Ignored *)
+      {| gsmsr_log := []; gsmsr_data := Ok _ _ gsm |}
   | GSMDT_TRANS_TLBI tlbi_data =>
-      step_tlbi trans.(gsmt_thread_identifier) tlbi_data st
+      step_tlbi trans.(gsmt_thread_identifier) tlbi_data gsm
   | GSMDT_TRANS_MSR msr_data =>
-      step_msr trans.(gsmt_thread_identifier) msr_data st
+      step_msr trans.(gsmt_thread_identifier) msr_data gsm
   | GSMDT_TRANS_HINT hint_data =>
-      step_hint trans.(gsmt_thread_identifier) hint_data st
+      step_hint trans.(gsmt_thread_identifier) hint_data gsm
   | GSMDT_TRANS_LOCK lock_data =>
-      step_lock trans.(gsmt_thread_identifier) lock_data st
+      step_lock trans.(gsmt_thread_identifier) lock_data gsm
   end.
 
 Definition memory_init := {|
@@ -53,12 +53,12 @@ Definition memory_init := {|
 Fixpoint all_steps_aux
   (transitions : list ghost_simplified_model_transition)
   (logs : list log_element)
-  (st : ghost_simplified_memory) :
+  (gsm : ghost_simplified_model) :
   ghost_simplified_model_result :=
   match transitions with
-    | [] => {| gsmsr_log := logs; gsmsr_data := Ok _ _ st; |}
+    | [] => {| gsmsr_log := logs; gsmsr_data := Ok _ _ gsm; |}
     | h :: t =>
-      match take_step h st with
+      match take_step h gsm with
         | {| gsmsr_log := logs_next; gsmsr_data := Ok _ _ st_next |} =>
             all_steps_aux t (logs_next ++ logs) st_next
         | {| gsmsr_log := logs_next; gsmsr_data := Error _ _ f |} =>
